src/Util/ParserInstances.v
@@ -11,6 +11,7 @@ From ExtLib Require Import
      Structures.Monoid.
 Import MonadNotation.
 From HTTP2 Require Import
+     HPACK.HPACKTypes
      Types
      Util.ByteVector
      Util.Parser
@@ -20,10 +21,15 @@ Import VectorNotations.
 
 Record parser (a : Type) := mkParser {
   run_parser : stateT bytes (sum HTTP2Error) a;
-}.
+                              }.
+Record HPACK_parser (a : Type) := mkHPACKParser {
+  run_HPACK_parser : stateT bytes (sum HPACKError) a;
+                                      }.
 
 Arguments mkParser {a}.
 Arguments run_parser {a}.
+Arguments mkHPACKParser {a}.
+Arguments run_HPACK_parser {a}.
 
 Instance Monad_parser : Monad parser := {
   ret _ a := mkParser (ret a);
@@ -31,8 +37,19 @@ Instance Monad_parser : Monad parser := {
     mkParser (run_parser p >>= fun x => run_parser (q x))%monad;
 }.
 
+Instance Monad_HPACK_parser : Monad HPACK_parser := {
+  ret _ a := mkHPACKParser (ret a);
+  bind _ _ p q :=
+    mkHPACKParser (run_HPACK_parser p >>= fun x => run_HPACK_parser (q x))%monad;
+}.
+
+
 Instance MError_parser : MError HTTP2Error parser := {
   throw _ e := mkParser (lift (inl e));
+}.
+
+Instance MError_HPACK_parser : MError HPACKError HPACK_parser := {
+  throw _ e := mkHPACKParser (lift (inl e));
 }.
 
 Instance MParser_parser : MParser byte parser := {
@@ -41,6 +58,17 @@ Instance MParser_parser : MParser byte parser := {
     match s with
     | "" =>
       lift (inl (ConnectionError FrameSizeError "not enough bytes"))
+    | c ::: s => MonadState.put s;; ret c
+    end
+  )%monad;
+}.
+
+Instance MParser_HPACK_parser : MParser byte HPACK_parser := {
+  get_token := mkHPACKParser (
+    s <- MonadState.get;;
+    match s with
+    | "" =>
+      lift (inl (decodeError "not enough bytes"))
     | c ::: s => MonadState.put s;; ret c
     end
   )%monad;
