src/HPACK/HPACKDecode.v
@@ -1,17 +1,25 @@
-From Coq Require Import String BinNat Ascii BinNatDef.
+From Coq Require Import String BinNat Ascii BinNatDef Vector.
+From HTTP2 Require Import
+     Equiv
+     Types
+     Util.BitVector
+     Util.ByteVector
+     Util.Parser
+     Util.VectorUtil
+     Util.StringUtil. 
 From HTTP2.HPACK Require Import HPACKTypes HPACKTables.
-From HTTP2.HPACK.Util Require Import HPACKOptionE.
 From ExtLib Require Import Monads.
 Import MonadNotation.
+Import Vector.VectorNotations.
 Open Scope N_scope.
 Open Scope string_scope.
-
+Open Scope monad_scope.
 
 (* Decodes a string to an integer where at least the first octet (ascii) is 
    assumed to be an encoded integer. The prefix is a value of n bits.
     https://tools.ietf.org/html/rfc7541#section-5.1
 
-Pseudocode to decode an integer I is as follows:
+Pseudocode to decode an integer I with an N bit prefix is as follows:
 
 decode I from the next N bits
 if I < 2^N - 1, return I
@@ -24,101 +32,79 @@ else
     while B & 128 == 128
     return I
  *)
-Fixpoint decode_integer_h (M:N) (s:string) : OptionE (N * string) :=
-  match s with
-  | EmptyString => inl decodeError
-  | String a s' =>
-    let B := N_of_ascii a in
-    let I := (BinNatDef.N.land B 127) * 2^M in
-    if N.land B 128 =? 128
-    then e <- decode_integer_h (M + 7) s' ;;
-         ret (I + fst e, snd e)
-    else ret (I, s')
-  end.
+Fixpoint decode_integer_h {m:Tycon} `{Monad m} `{MError HPACKError m}
+           `{MParser byte m} (M:N) : m N :=
+  a <- get_byte ;;
+  let B := (N_of_ascii a) in
+  let I := (BinNatDef.N.land B 127) * 2^M in
+  if N.land B 128 =? 128
+  then (*e <- decode_integer_h (M + 7) ;;
+       ret (I + e)*) ret I
+  else ret I.
 
-Definition decode_integer (prefix:N) (n:N) (s:string) : OptionE (N * string) :=
-  if prefix <? 2^n - 1 then ret (prefix, s)
-  else a <- decode_integer_h 0 s ;;
-       ret (prefix + fst a, snd a).
+Definition decode_integer {m:Tycon} `{Monad m} `{MError HPACKError m}
+           `{MParser byte m} (prefix:N) (n:N) : m N :=
+  if prefix <? 2^n - 1 then ret prefix
+  else a <- decode_integer_h 0 ;;
+       ret (prefix + a).
 
 
 (*  https://tools.ietf.org/html/rfc7541#section-5.2 *)
 (* Decodes the huffman encoded string s *)
-Definition decode_hstring (s:string) : OptionE string := ret "".
+Definition decode_hstring {m:Tycon} `{Monad m} `{MError HPACKError m}
+           `{MParser byte m} (s:string) : m string := ret "".
 
-(* Splits the string, returning the first n octets in the first of the pair, the 
-   rest in the second. *)
-Fixpoint get_n_string (s:string) (n:N) : OptionE (string * string) :=
-  match s with
-  | EmptyString => if n =? 0 then ret ("", "") else inl decodeError
-  | String a s' => if n =? 0 then ret ("", s')
-                  else e <- get_n_string s' (N.pred n) ;;
-                       ret (String a (fst e), snd e)
-  end.
-
-(* Decodes an encoded string to a raw string, returning the decoded string as the
-   first of the pair, and the rest as the second. *)
-Definition decode_string (s:string) : OptionE (string * string) :=
-  match s with
-  | EmptyString => inl decodeError
-  | String a s' =>
-    let n := N_of_ascii a in
-    let H := N.land n 128 in
-    let prefix := N.land n 127 in
-    v1 <- decode_integer prefix 7 s' ;;
-    v2 <- get_n_string (snd v1) (fst v1) ;;
-    if BinNat.N.eqb H 128 then ret v2
-    else s'' <- decode_hstring (fst v2) ;; ret (s'', snd v2)
-  end.
+(* Decodes an encoded string to a raw string. *)
+Definition decode_string {m:Tycon} `{Monad m} `{MError HPACKError m}
+           `{MParser byte m} : m string :=
+  a <- get_byte ;;
+  let n := N_of_ascii a in
+  let prefix := N.land n 127 in
+  len <- decode_integer prefix 7 ;;
+  s <- get_bytes_N len ;;
+  let H := N.land n 128 in
+  if BinNat.N.eqb H 128 then decode_hstring s
+  else ret s.
 
 (* https://tools.ietf.org/html/rfc7541#section-6 *)
-(* Decodes a header field representation, returning the rest of the string leftover *)
-Definition decode_HFR (s:string) : OptionE (HeaderFieldRepresentation * string) :=
-  match s with
-  | EmptyString => inl decodeError
-  | String a s' =>
-    let octet := N_of_ascii a in
-    let bit0 := N.land octet 128 in
-    (* https://tools.ietf.org/html/rfc7541#section-6.1 *)
-    if bit0 =? 128 then fmap (decode_integer (N.land octet 127) 7 s')
-                             (fun '(n, s) => ret (IndexedHF n, s))
+(* Decodes a header field representation *)
+Definition decode_HFR {m:Tycon} `{Monad m} `{MError HPACKError m}
+           `{MParser byte m} : m HeaderFieldRepresentation :=
+  a <- get_byte ;;
+  let octet := N_of_ascii a in
+  let bit0 := N.land octet 128 in
+  (* https://tools.ietf.org/html/rfc7541#section-6.1 *)
+  if bit0 =? 128 then n <- decode_integer (N.land octet 127) 7;;
+                      ret (IndexedHF n)
+  else
+    let bit1 := N.land octet 64 in
+    (* https://tools.ietf.org/html/rfc7541#section-6.2.1 *)
+    if bit1 =? 1
+    then v <- decode_integer (N.land octet 63) 6;;
+         if v =? 0 then v1 <- decode_string;;
+                        v2 <- decode_string;;
+                        ret (LHFIncrementNewName v1 v2)
+           else v1 <- decode_string;;
+                ret (LHFIncrementIndexedName v v1)
     else
-      let bit1 := N.land octet 64 in
-      (* https://tools.ietf.org/html/rfc7541#section-6.2.1 *)
-      if bit1 =? 1
-      then v <- decode_integer (N.land octet 63) 6 s' ;;
-           if fst v =? 0 then v1 <- decode_string (snd v) ;;
-                              v2 <- decode_string (snd v1) ;;
-                              ret (LHFIncrementNewName (fst v1) (fst v2), snd v2)
-           else v1 <- decode_string (snd v) ;;
-                ret (LHFIncrementIndexedName (fst v) (fst v1), snd v1)
+      (* https://tools.ietf.org/html/rfc7541#section-6.3 *)
+      let bit2 := N.land octet 32 in
+      if bit2 =? 32 then n <- decode_integer (N.land octet 31) 5;;
+                         ret (DTableSizeUpdate n)
       else
-        (* https://tools.ietf.org/html/rfc7541#section-6.3 *)
-        let bit2 := N.land octet 32 in
-        if bit2 =? 32 then fmap (decode_integer (N.land octet 31) 5 s')
-                                (fun '(n, s) => ret (DTableSizeUpdate n, s))
+        (* https://tools.ietf.org/html/rfc7541#section-6.2.3 *)
+        let bit3 := N.land octet 16 in
+        if bit3 =? 16 then v <- decode_integer (N.land octet 15) 4;;
+                           if v =? 0 then v1 <- decode_string;;
+                                          v2 <- decode_string;;
+                                          ret (LHFNeverIndexNewName v1 v2)
+                           else v1 <- decode_string;;
+                                ret (LHFNeverIndexIndexedName v v1)
         else
-          (* https://tools.ietf.org/html/rfc7541#section-6.2.3 *)
-          let bit3 := N.land octet 16 in
-          if bit3 =? 16 then v <- decode_integer (N.land octet 15) 4 s' ;;
-                             if fst v =? 0 then v1 <- decode_string (snd v) ;;
-                                                v2 <- decode_string (snd v1) ;;
-                                                ret (LHFNeverIndexNewName (fst v1)
-                                                                          (fst v2),
-                                                     snd v2)
-                             else v1 <- decode_string (snd v) ;;
-                                  ret (LHFNeverIndexIndexedName (fst v)
-                                                                (fst v1), snd v1)
-          else
-            (* https://tools.ietf.org/html/rfc7541#section-6.2.2 *)
-            v <- decode_integer (N.land octet 15) 4 s' ;;
-            if fst v =? 0 then v1 <- decode_string (snd v) ;;
-                               v2 <- decode_string (snd v1) ;;
-                               ret (LHFWithoutIndexNewName (fst v1) (fst v2), snd v2)
-              else v1 <- decode_string (snd v) ;;
-                   ret (LHFWithoutIndexIndexedName (fst v) (fst v1), snd v1)
-  end.
-
-Definition decode_HL (hl:HeaderList) : OptionE HeaderBlock :=
-  List.fold_left (fun acc s => a <- decode_HFR s ;; h <- acc ;;
-                            ret (fst a :: h)) hl (ret (nil%list)).
+          (* https://tools.ietf.org/html/rfc7541#section-6.2.2 *)
+          v <- decode_integer (N.land octet 15) 4;;
+          if v =? 0 then v1 <- decode_string;;
+                         v2 <- decode_string;;
+                         ret (LHFWithoutIndexNewName v1 v2)
+          else v1 <- decode_string;;
+               ret (LHFWithoutIndexIndexedName v v1).
