src/HPACK/HPACKProcessor.v
@@ -1,4 +1,5 @@
-From HTTP2.HPACK Require Import HPACKTypes HPACKTables Util.HPACKOptionE.
+From HTTP2.HPACK Require Import HPACKTypes HPACKTables.
+From HTTP2.Util Require Import Parser.
 From Coq Require Import Basics.
 From ExtLib Require Import Monads.
 Import MonadNotation.
@@ -7,8 +8,8 @@ Import MonadNotation.
 (* Takes a Header Field Representation (which is part of a Header Block) and 
    a dynamic table, and processes the hfr, returning either an error,
    or a potentially mutated dynamic table. *)
-Definition processHFR (hfr:HeaderFieldRepresentation) (dynamic_table:DTable)
-  : OptionE DTable :=
+Definition processHFR {m:Tycon} `{Monad m} `{MError HPACKError m}
+           (hfr:HeaderFieldRepresentation) (dynamic_table:DTable) : m DTable :=
   match hfr with
   | LHFIncrementIndexedName x s2 =>
     s <- index_into_tables x dynamic_table ;;
